svc enc-ni, enc-low-equiv is side-channel free... There are 3 timeouts / violations left in enc-ni-enter

verified/secprop/sec_prop.s.dfy
@@ -70,13 +70,13 @@ predicate enc_eqentry(e1:PageDbEntryTyped, e2:PageDbEntryTyped)
     match e1
         case Addrspace(_,_,_,_,_)
             => e2.Addrspace? && e1.(shatrace := e2.shatrace) == e2 // shatrace is irrelevant
-        case L1PTable(_) => e1 == e2
-        case L2PTable(_) => e1 == e2
         case Dispatcher(_,_,_,_,_) => 
             e2.Dispatcher? && e2.entered == e1.entered &&
                 e2.entrypoint == e1.entrypoint
-        case DataPage(_) => e2.DataPage?
-        case SparePage => e2.SparePage?
+        case L1PTable(_) => e2.L1PTable?
+        case L2PTable(_) => e2.DataPage? || e2.SparePage? || e2.LtPTable? 
+        case DataPage(_) => e2.DataPage? || e2.SparePage? || e2.L2PTable?
+        case SparePage   => e2.DataPage? || e2.SparePage? || e2.L2PTable?
 }
 
 
